README.md
@@ -2,7 +2,7 @@
 
 This is an in-progress, open-source book by [Adam Chlipala](http://adam.chlipala.net/) simultaneously introducing [the Coq proof assistant](http://coq.inria.fr/) and techniques for proving correctness of programs.  That is, the game is doing completely rigorous, machine-checked mathematical proofs, showing that programs meet their specifications.
 
-Just run `make` here to build everything, including the book `frap.pdf` and the accompanying Coq source modules.
+Just run `make` here to build everything, including the book `frap.pdf` and the accompanying Coq source modules.  Alternatively, run `make lib' to build just the book library, not the chapter example files or PDF.
 
 # Code associated with the different chapters
 
@@ -18,3 +18,4 @@ Just run `make` here to build everything, including the book `frap.pdf` and the 
 * Chapter 11: `DeepAndShallowEmbeddings.v`
 * Chapter 12: `SeparationLogic.v`
 * Chapter 13: `SharedMemory.v`
+* Chapter 14: `ConcurrentSeparationLogic.v`
